revm:add clone for EofBody

CoqOfRust/alloc/links/alloc.v
@@ -10,4 +10,8 @@ Module Global.
     Φ := Ty.path "alloc::alloc::Global";
     φ := to_value;
   }.
+
+  Definition of_ty : OfTy.t (Ty.path "alloc::alloc::Global").
+  Proof. eapply OfTy.Make with (A := t); reflexivity. Defined.
+  Smpl Add apply of_ty : of_ty.
 End Global.
