CoqOfRust/core/links/clone.v
@@ -1,5 +1,6 @@
 Require Import CoqOfRust.CoqOfRust.
 Require Import links.M.
+Require Import core.clone.
 
 (*
     pub trait Clone: Sized {
@@ -23,3 +24,26 @@ Module Clone.
     (* TODO: add [clone_from] *)
   }.
 End Clone.
+
+Module Impl_Clone_for_bool.
+  Definition run_clone : clone.Clone.Run_clone bool.
+  Proof.
+    eexists; split.
+    { eapply IsTraitMethod.Defined.
+      { apply clone.impls.Impl_core_clone_Clone_for_bool.Implements. }
+      { reflexivity. }
+    }
+    { intros.
+      run_symbolic.
+    }
+  Defined.
+
+
+  Definition run : clone.Clone.Run bool.
+  Proof.
+    constructor.
+    { (* clone *)
+      exact run_clone.
+    }
+  Defined.
+End Impl_Clone_for_bool.
